首先考虑二维的情况
$$
A=\left( \begin{matrix}
a_{1,1} & a_{1,2} \\
a_{2,1} & a_{2,2}
\end{matrix} \right) \qquad \mathbf{x} = \left( \begin{matrix}
x_{1} \\
x_{2}
\end{matrix} \right) \in R^2
$$
且
$$
\begin{align}
f(\mathbf{x}) & =\mathbf{x}^TA\mathbf{x} \\
 & = \left( \begin{matrix} x_{1} & x_{2} \end{matrix} \right) \left( \begin{matrix} a_{1,1} & a_{1,2} \\ a_{2,1} & a_{2,2} \end{matrix} \right) \left( \begin{matrix} x_{1} \\ x_{2} \end{matrix} \right) \\
 & = \left( \begin{matrix} x_{1} & x_{2} \end{matrix} \right) \left( \begin{matrix} x_{1}a_{1,1}+x_{2}a_{1,2} \\ x_{1}a_{2,1}+x_{2}a_{2,2} \end{matrix} \right)  \\
 & = x_{1}^2a_{1,1}+x_{1}x_{2}(a_{1,2}+a_{2,1})+x_{2}^2a_{2,2}
\end{align}
$$
求证
$$\nabla f(\mathbf{x})= A\mathbf{x}+A^T\mathbf{x}$$
证明
$$\begin{align}
\nabla f(\mathbf{x}) & =\left( \begin{matrix}
\frac{{\partial f(\mathbf{x})}}{\partial x_{1}} \\
\frac{{\partial f(\mathbf{x})}}{\partial x_{2}}
\end{matrix} \right) \\
 & =\left( \begin{matrix} 2x_{1}a_{1,1} + x_{2}(a_{1,2}+a_{2,1}) \\         2x_{2}a_{2,2} + x_{1}(a_{1,2}+a_{2,1}) \end{matrix} \right)  \\
	 & = \left( \begin{matrix} x_{1}a_{1,1}+x_{2}a_{1,2} \\ x_{1}a_{2,1} + x_{2}a_{2,2} \end{matrix} \right) +\left( \begin{matrix} x_{1}a_{1,1}+x_{2}a_{2,1} \\ x_{1}a_{1,2} + x_{2}a_{2,2} \end{matrix} \right)  \\
 & = \left( \begin{matrix} a_{1,1} & a_{1,2} \\ a_{2,1} &  a_{2,2} \end{matrix} \right) \left( \begin{matrix} x_{1} \\ x_{2} \end{matrix} \right) + \left( \begin{matrix} a_{1,1} & a_{2,1} \\ a_{1,2} &  a_{2,2} \end{matrix} \right) \left( \begin{matrix} x_{1} \\ x_{2} \end{matrix} \right) \\
 & =A\mathbf{x}+A^T\mathbf{x}
\end{align}$$