更普遍的形式
$$
A = \left( \begin{matrix}
    a_{1,1} & \dots  & a_{1,d} \\
	\vdots &  & \vdots \\
    a_{d,1} & \dots & a_{d,d} \end{matrix} \right)  \qquad 
\mathbf{x} = \left( \begin{matrix}
    x_{1} \\
	\vdots \\
    x_{d}
    \end{matrix} \right) 
$$
定义
$$
\begin{align}
f(\mathbf{x}) & =\mathbf{x}^TA\mathbf{x} \\
 & = \sum_{i,j=1}^da_{i,j}x_{i}x_{j}
\end{align}
$$
求证
$$
\nabla f(\mathbf{x})=A\mathbf{x}+A^T\mathbf{x}
$$
证明
$$\begin{align}
\nabla f(\mathbf{x}) & =\left( \begin{matrix}
    \frac{\partial f(x_{1})}{\partial x_{1}} \\
    \vdots \\
    \frac{\partial f(x_{d})}{\partial x_{d}}
    \end{matrix} \right)  \\
& = \left( \begin{matrix}
	    \frac{\partial \left( \sum_{j=1}^na_{1,j}x_{1}x_{j} \right)}{\partial x_{1}} \\
    \vdots \\
    \frac{\partial \left( \sum_{j=1}^na_{d,j}x_{d}x_{j} \right)}{\partial x_{d}}
    \end{matrix} \right)  \\
& = \left( \begin{matrix}
    2a_{1,1}x_{1} +\sum_{i=1}^da_{i,1}x_{i}\delta_{1,i} + \sum_{j=1}^da_{1,j}x_{j}\delta_{1,j} \\
    \vdots \\
    2a_{d,d}x_{d} +\sum_{i=1}^da_{i,d}x_{i}\delta_{d,i} +\sum_{j=1}^da_{d,j}x_{j}\delta_{d,j}
    \end{matrix} \right)   \\
& =\left( \begin{matrix}
    \sum_{j=1}^da_{1,j}x_{j} \\
    \vdots \\
    \sum_{j=1}^da_{d,j}x_{j}
    \end{matrix} \right) + \left( \begin{matrix}
    \sum_{i=1}^da_{i,1}x_{i} \\
    \vdots \\
    \sum_{i=1}^da_{i,d}x_{i}
    \end{matrix} \right) \\
& =A\mathbf{x}+A^T\mathbf{x}
\end{align}$$